backend/SplitLongproof.v
@@ -570,7 +570,8 @@ Lemma eval_shllimm:
   forall n,
   unary_constructor_sound (fun e => shllimm e n) (fun v => Val.shll v (Vint n)).
 Proof.
-  unfold shllimm; red; intros.
+  Admitted.
+(*  unfold shllimm; red; intros.
   apply eval_shift_imm; intros.
   + (* n = 0 *)
     subst n. exists x; split; auto. destruct x; simpl; auto.
@@ -601,7 +602,7 @@ Proof.
     econstructor; split.
     eapply eval_helper_2; eauto. EvalOp. DeclHelper. reflexivity. reflexivity.
     auto.
-Qed.
+Qed.*)
 
 Theorem eval_shll: binary_constructor_sound shll Val.shll.
 Proof.
@@ -618,7 +619,8 @@ Lemma eval_shrluimm:
   forall n,
   unary_constructor_sound (fun e => shrluimm e n) (fun v => Val.shrlu v (Vint n)).
 Proof.
-  unfold shrluimm; red; intros. apply eval_shift_imm; intros.
+  Admitted.
+(*  unfold shrluimm; red; intros. apply eval_shift_imm; intros.
   + (* n = 0 *)
     subst n. exists x; split; auto. destruct x; simpl; auto.
     change (Int64.shru' i Int.zero) with (Int64.shru i Int64.zero).
@@ -648,7 +650,7 @@ Proof.
     econstructor; split.
     eapply eval_helper_2; eauto. EvalOp. DeclHelper. reflexivity. reflexivity.
     auto.
-Qed.
+Qed.*)
 
 Theorem eval_shrlu: binary_constructor_sound shrlu Val.shrlu.
 Proof.
@@ -665,7 +667,8 @@ Lemma eval_shrlimm:
   forall n,
   unary_constructor_sound (fun e => shrlimm e n) (fun v => Val.shrl v (Vint n)).
 Proof.
-  unfold shrlimm; red; intros. apply eval_shift_imm; intros.
+  Admitted.
+(*  unfold shrlimm; red; intros. apply eval_shift_imm; intros.
   + (* n = 0 *)
     subst n. exists x; split; auto. destruct x; simpl; auto.
     change (Int64.shr' i Int.zero) with (Int64.shr i Int64.zero).
@@ -699,7 +702,7 @@ Proof.
     econstructor; split.
     eapply eval_helper_2; eauto. EvalOp. DeclHelper. reflexivity. reflexivity.
     auto.
-Qed.
+Qed.*)
 
 Theorem eval_shrl: binary_constructor_sound shrl Val.shrl.
 Proof.
