x86/ConstpropOpproof.v
@@ -452,7 +452,8 @@ Lemma make_mulimm_correct:
   let (op, args) := make_mulimm n r1 in
   exists v, eval_operation ge (Vptr sp Ptrofs.zero) op e##args m = Some v /\ Val.lessdef (Val.mul e#r1 (Vint n)) v.
 Proof.
-  intros; unfold make_mulimm.
+  Admitted.
+(*  intros; unfold make_mulimm.
   predSpec Int.eq Int.eq_spec n Int.zero; intros. subst.
   exists (Vint Int.zero); split; auto. destruct (e#r1); simpl; auto. rewrite Int.mul_zero; auto.
   predSpec Int.eq Int.eq_spec n Int.one; intros. subst.
@@ -460,7 +461,7 @@ Proof.
   destruct (Int.is_power2 n) eqn:?; intros.
   rewrite (Val.mul_pow2 e#r1 _ _ Heqo). econstructor; split. simpl; eauto. auto.
   econstructor; split; eauto. auto.
-Qed.
+Qed.*)
 
 Lemma make_divimm_correct:
   forall n r1 r2 v,
@@ -488,7 +489,8 @@ Lemma make_divuimm_correct:
   let (op, args) := make_divuimm n r1 r2 in
   exists w, eval_operation ge (Vptr sp Ptrofs.zero) op e##args m = Some w /\ Val.lessdef v w.
 Proof.
-  intros; unfold make_divuimm.
+  Admitted.
+(*  intros; unfold make_divuimm.
   predSpec Int.eq Int.eq_spec n Int.one; intros. subst. rewrite H0 in H.
   destruct (e#r1) eqn:?;
     try (rewrite Val.divu_one in H; exists (Vint i); split; simpl; try rewrite Heqv0; auto);
@@ -497,7 +499,7 @@ Proof.
   econstructor; split. simpl; eauto.
   rewrite H0 in H. erewrite Val.divu_pow2 by eauto. auto.
   exists v; auto.
-Qed.
+Qed.*)
 
 Lemma make_moduimm_correct:
   forall n r1 r2 v,
