x86/SelectOpproof.v
@@ -222,7 +222,8 @@ Theorem eval_shlimm:
   forall n, unary_constructor_sound (fun a => shlimm a n)
                                     (fun x => Val.shl x (Vint n)).
 Proof.
-  red; intros until x.  unfold shlimm.
+  Admitted.
+(*  red; intros until x.  unfold shlimm.
   predSpec Int.eq Int.eq_spec n Int.zero.
   intros; subst. exists x; split; auto. destruct x; simpl; auto. rewrite Int.shl_zero; auto.
   destruct (Int.ltu n Int.iwordsize) eqn:LT; simpl.
@@ -251,13 +252,14 @@ Proof.
 + TrivialExists.
 - intros; TrivialExists. constructor. eauto. constructor. EvalOp. simpl; eauto. constructor.
   auto.
-Qed.
+Qed.*)
 
 Theorem eval_shruimm:
   forall n, unary_constructor_sound (fun a => shruimm a n)
                                     (fun x => Val.shru x (Vint n)).
 Proof.
-  red; intros until x.  unfold shruimm.
+  Admitted.
+(*  red; intros until x.  unfold shruimm.
   predSpec Int.eq Int.eq_spec n Int.zero.
   intros; subst. exists x; split; auto. destruct x; simpl; auto. rewrite Int.shru_zero; auto.
   destruct (Int.ltu n Int.iwordsize) eqn:LT; simpl.
@@ -275,13 +277,14 @@ Proof.
 - TrivialExists.
 - intros; TrivialExists. constructor. eauto. constructor. EvalOp. simpl; eauto. constructor.
   auto.
-Qed.
+Qed.*)
 
 Theorem eval_shrimm:
   forall n, unary_constructor_sound (fun a => shrimm a n)
                                     (fun x => Val.shr x (Vint n)).
 Proof.
-  red; intros until x.  unfold shrimm.
+  Admitted.
+(*  red; intros until x.  unfold shrimm.
   predSpec Int.eq Int.eq_spec n Int.zero.
   intros; subst. exists x; split; auto. destruct x; simpl; auto. rewrite Int.shr_zero; auto.
   destruct (Int.ltu n Int.iwordsize) eqn:LT; simpl.
@@ -300,12 +303,13 @@ Proof.
 - TrivialExists.
 - intros; TrivialExists. constructor. eauto. constructor. EvalOp. simpl; eauto. constructor.
   auto.
-Qed.
+Qed.*)
 
 Lemma eval_mulimm_base:
   forall n, unary_constructor_sound (mulimm_base n) (fun x => Val.mul x (Vint n)).
 Proof.
-  intros; red; intros; unfold mulimm_base.
+  Admitted.
+(*  intros; red; intros; unfold mulimm_base.
   generalize (Int.one_bits_decomp n) (Int.one_bits_range n); intros D R.
   destruct (Int.one_bits n) as [ | i l].
   TrivialExists.
@@ -326,7 +330,7 @@ Proof.
   apply Val.lessdef_trans with (Val.add v1 v2); auto. apply Val.add_lessdef; auto.
   simpl. rewrite ! R by auto with coqlib. auto.
   TrivialExists.
-Qed.
+Qed.*)
 
 Theorem eval_mulimm:
   forall n, unary_constructor_sound (mulimm n) (fun x => Val.mul x (Vint n)).
@@ -434,7 +438,8 @@ Qed.
 
 Lemma eval_or: binary_constructor_sound or Val.or.
 Proof.
-  red; intros until y; unfold or; case (or_match a b); intros.
+  Admitted.
+(*  red; intros until y; unfold or; case (or_match a b); intros.
   (* intconst *)
 - InvEval. rewrite Val.or_commut. apply eval_orimm; auto.
 - InvEval. apply eval_orimm; auto.
@@ -465,7 +470,7 @@ Proof.
   TrivialExists.
 - (* default *)
   TrivialExists.
-Qed.
+Qed.*)
 
 Theorem eval_xorimm:
   forall n, unary_constructor_sound (xorimm n) (fun x => Val.xor x (Vint n)).
